src/extraction/FStar.Extraction.ML.UEnv.fst
@@ -449,8 +449,8 @@ let extend_bv (g:uenv) (x:bv) (t_x:mltyscheme) (add_unit:bool)
               else if add_unit
               then with_ty MLTY_Top <| MLE_App(with_ty MLTY_Top mlx, [ml_unit])
               else with_ty ml_ty mlx in
-    let t_x = if add_unit then pop_unit t_x else t_x in
-    let exp_binding = {exp_b_name=mlident; exp_b_expr=mlx; exp_b_tscheme=t_x } in
+    let eff, t_x = if add_unit then pop_unit t_x else E_PURE, t_x in
+    let exp_binding = {exp_b_name=mlident; exp_b_expr=mlx; exp_b_tscheme=t_x; exp_b_eff=eff } in
     let gamma = Bv(x, Inr exp_binding)::g.env_bindings in
     let tcenv = TypeChecker.Env.push_binders g.env_tcenv (binders_of_list [x]) in
     {g with env_bindings=gamma; env_mlident_map = mlident_map; env_tcenv=tcenv}, mlident, exp_binding
@@ -497,8 +497,8 @@ let extend_fv (g:uenv) (x:fv) (t_x:mltyscheme) (add_unit:bool)
         let mlsymbol = snd mlpath in
         let mly = MLE_Name mlpath in
         let mly = if add_unit then with_ty MLTY_Top <| MLE_App(with_ty MLTY_Top mly, [ml_unit]) else with_ty ml_ty mly in
-        let t_x = if add_unit then pop_unit t_x else t_x in
-        let exp_binding = {exp_b_name=mlsymbol; exp_b_expr=mly; exp_b_tscheme=t_x } in
+        let eff, t_x = if add_unit then pop_unit t_x else E_PURE, t_x in
+        let exp_binding = {exp_b_name=mlsymbol; exp_b_expr=mly; exp_b_tscheme=t_x; exp_b_eff=eff } in
         let gamma = Fv(x, exp_binding)::g.env_bindings in
         let mlident_map = BU.psmap_add g.env_mlident_map mlsymbol "" in
         {g with env_bindings=gamma; env_mlident_map=mlident_map}, mlsymbol, exp_binding
